proof/format_proof.v
@@ -7,6 +7,7 @@ Require Import printer.verified_printer.Format.
 Require Import Coq.Strings.Ascii.
 Require Import format_specs.
 Require Import format_std_proof.
+Require Import list_specs.
 
 Lemma less_components_fact1: 
   forall (x y : nat), 
