proof/list_specs.v
@@ -1,0 +1,99 @@
+Require Import HahnBase.
+
+Require Import VST.floyd.proofauto.
+Require Import VST.floyd.library.
+Require Import printer.printer_files.compiled_format.
+Require Import printer.verified_printer.Format.
+Require Import printer.verified_printer.FormatTrivial.
+Require Import Coq.Strings.Ascii.
+Require Import format_specs.
+
+Definition t_flist := Tstruct _format_list noattr.
+
+Fixpoint listrepf (sigma: list t) (p: val) : mpred :=
+ match sigma with
+ | G::hs =>
+    EX x:val, EX y: val,
+    malloc_token Ews t_format y *
+    mformat G y *
+    malloc_token Ews t_flist p * 
+    data_at Ews t_flist ((y, x) : @reptype CompSpecs t_flist) p *
+    listrepf hs x
+ | nil =>
+    !! (<< LIST_NULL_PTR : p = nullval >> ) && emp
+ end.
+
+Arguments listrepf sigma p : simpl never.
+
+Lemma listrepf_local_facts sigma p :
+   listrepf sigma p |--
+   !! (<< LIST_PTR_FACT : is_pointer_or_null p /\ (p=nullval <-> sigma=nil) >>).
+Proof.
+  intros.
+  revert p; induction sigma; intros p.
+  { unfold listrepf. unnw. entailer!. split; auto. }
+  unff listrepf.
+  destruct a. entailer. unnw. entailer!.
+  split; ins.
+  subst. eapply field_compatible_nullval; eauto.
+Qed.
+#[export] Hint Resolve listrepf_local_facts : saturate_local.
+
+Lemma listrepf_valid_pointer sigma p :
+   listrepf sigma p |-- valid_pointer p.
+Proof.
+  intros.
+  unfold listrepf. destruct sigma; simpl; unnw.
+  { entailer!. }
+  Intros x y. auto with valid_pointer.
+Qed.
+#[export] Hint Resolve listrepf_valid_pointer : valid_pointer.
+
+Fixpoint lsegf (sigma: list t) (x z: val) : mpred :=
+  match sigma with
+  | nil => !! (<< LSEG_PTR_FACT : x = z >>) && emp
+  | G::hs => EX h: val, EX y:val, 
+      malloc_token Ews t_format y *
+      mformat G y *
+      malloc_token Ews t_flist x * 
+      data_at Ews t_flist ((y, h) : @reptype CompSpecs t_flist) x *
+      lsegf hs h z
+  end.
+
+Arguments lsegf sigma x z : simpl never.
+
+Definition good_format (G : t) (w h : Z) : Prop :=
+   (total_width G <= Z.to_nat w)%nat /\ (G.(height) <= Z.to_nat h)%nat.
+
+Definition good_format_list (sigma : list t) (w h : Z) : Prop :=
+  Forall (fun G => good_format G w h) sigma.
+
+Definition beside_doc_spec : ident * funspec :=
+ DECLARE _beside_doc
+  WITH fs1 : list t, fs2 : list t, p1 : val, p2 : val, w : Z, h : Z
+  PRE [ tuint, tuint, tptr t_flist, tptr t_flist ]
+    PROP (good_format_list fs1 w h; good_format_list fs2 w h;
+         0 <= 4 * w <= Int.max_unsigned;
+         0 <= 4 * h <= Int.max_unsigned)
+   PARAMS(Vint (Int.repr w); Vint (Int.repr h); p1; p2)
+    SEP (listrepf fs1 p1; listrepf fs2 p2)
+  POST [ tptr t_flist ]
+    EX p: val, EX sigma: list t,
+    PROP (good_format_list sigma w h;
+            sigma = filter (fun G => (G.(height) <=? (Z.to_nat h))%nat) (besideDoc (Z.to_nat w) fs1 fs2))
+   RETURN(p)
+   SEP (listrepf sigma p).
+
+Definition Gprog : funspecs :=
+        ltac:(with_library prog [
+                   max_spec; strlen_spec; strcpy_spec; strcat_spec;
+                   list_copy_spec; less_components_spec; is_less_than_spec; 
+                   empty_spec; line_spec; sp_spec; 
+                   get_applied_length_spec; format_copy_spec; get_list_tail_spec;
+                   mdw_add_above_spec; list_concat_spec; to_text_add_above_spec;
+                   new_list_spec; add_above_spec;
+                   flw_add_beside_spec; shift_list_spec; add_beside_spec; line_concats_spec;
+                   mdw_add_beside_spec; to_text_add_beside_spec;
+                   mdw_add_fill_spec; flw_add_fill_spec; to_text_add_fill_spec;
+                   llw_add_fill_spec; add_fill_spec; beside_doc_spec
+ ]).
