proof/list_trivial_proof.v
@@ -1,0 +1,13 @@
+
+Require Import HahnBase.
+
+Require Import VST.floyd.proofauto.
+Require Import VST.floyd.library.
+Require Import printer.printer_files.compiled_format.
+Require Import printer.verified_printer.Format.
+Require Import Coq.Strings.Ascii.
+Require Import format_specs.
+Require Import format_std_proof.
+Require Import format_proof.
+Require Import list_specs.
+Require Import format_combinator_proof.
